
- $p(x_i \mid s_i) = \frac{s_i^{x_i} \exp(-s_i)}{x_i!}$
- $p(\mathbf{x} \mid \mathbf{s}) = \prod_{i=1}^{n} p(x_i \mid s_i)$
- $p(s|x) \propto p(x|s) p(s)$
- $s=\int p(s|x)s\,ds$
- $\prod_{i=1}^Tp(t_i|s)$
- $x_t=\sum_{i=1}^T\mathbb{1}(t_i=t)$
- $p(\{i\}|s,T)=\begin{cases}\prod_{t=1}^Tp(i=i_t|s)&T=|\{i\}|\\0&T\neq |\{i\}|\end{cases}$
- $p(\{i\}|s,T)=\begin{cases}\prod_{i=1}^np(i|s)^{x_i}&T=|\{i\}|\\0&T\neq |\{i\}|\end{cases}$
- $p(i_t=i|s)=\frac{s_i}{\sum_{j=1}^ns_j}$
- $p(\{i\}|T)=\begin{cases}\prod_{t=1}^Tp(i=i_t|i_1,\ldots,i_{t-1},T)&T=|\{i\}|\\0&T\neq |\{i\}|\end{cases}$
- $p(i = i_t|i_1, \ldots, i_{t-1}, T) = p(i = i_t|x_{t-1})$
- $p(i = i_t|x_{t-1}) = \int p(s|x_{t-1})p(i_t = i|s, x_{t-1}) \, ds$
- $L(\theta) = -\sum_{k=1}^m \sum_{i=1}^n \ln f_i(x_{\text{inp}}^k; \theta) x_{\text{tar},i}^k$
- $L(\theta) = -\sum_{k=1}^m \frac{1}{n|x_{\text{tar}}^k|} \sum_{i=1}^n \ln f_i(x_{\text{inp}}^k; \theta) x_{\text{tar},i}^k$
